#+AUTHOR:
First we only consider *one play*
\begin{eqnarray}
G(P_{n}, w^{1}) = \sum_{i=1}^{S} \tilde{\theta_{i}} \tanh(\theta_{i} P_{n} + \theta_{i0}) + \tilde{\theta_{0}}
\end{eqnarray}

Where \(P_{n} = [p_{1}, p_{2}, p_{3}, ..., p_{n}]\), \(G(P_{n}, w^{1}) = [y_{1}, y_{2}, y_{3}, ..., y_{n}]\)

\(\forall{i} \in [1, ..., S]\), \(\theta_{i} P_{n} = (\theta_{i} p_{1}, \theta_{i} p_{2}, \theta_{i} p_{3}, ..., \theta_{i} p_{n})\),

So
\(\tanh(\theta_{i} P_{n} + \theta_{i0}) =
[\tanh(\theta_{i} p_{1} + \theta_{i0}),
\tanh(\theta_{i} p_{2} + \theta_{i0}),
\tanh(\theta_{i} p_{3} + \theta_{i0}),
...,
\tanh(\theta_{i} p_{n} + \theta_{i0})]\)

So \(\sum_{i=1}^{S} \tilde{\theta_{i}} \tanh(\theta_{i} P_{n} + \theta_{i0}) + \tilde{\theta_{0}} =
[\sum_{i=1}^{S} \tilde{\theta_{i}} \tanh(\theta_{i} p_{1} + \theta_{i0}) + \tilde{\theta_{0}},
\sum_{i=1}^{S} \tilde{\theta_{i}} \tanh(\theta_{i} p_{2} + \theta_{i0}) + \tilde{\theta_{0}},
...,
\sum_{i=1}^{S} \tilde{\theta_{i}} \tanh(\theta_{i} p_{n} + \theta_{i0}) + \tilde{\theta_{0}}] =
[y_{1}, y_{2}, ..., y_{n}]\).

Take \(y_{j}\), where \(j \in [1, ..., n]\) for example

\begin{eqnarray}
y_{j}  = \sum_{i=1}^{S} \tilde{\theta_{i}} \tanh(\theta_{i} p_{j} + \theta_{i0}) + \theta_{i0}
\end{eqnarray}

Calculate derivation for \(y_{j}\)
\begin{eqnarray}
\frac{\partial y_{j}}{\partial p_{j}} &=& \sum_{i=1}^{S} \tilde{\theta_{i}} \frac{\partial \tanh(\theta_{i} p_{j} + \theta_{i0})}{\partial p_{j}}  \\
\end{eqnarray}

                                      # &=& \sum_{i=1}^{S} \tilde{\theta_{i}} \theta_{i} \frac{\partial{}}{\partial{}} \\
                                      # &=& \sum_{i=1}^{S} \tilde{\theta_{i}} \theta_{i} (1 - \tanh^{2}(\theta_{i} p_{j} + \theta_{i0})) \\

Now let's consider the mapping between \(p_{j}\) and \(x_{j}\).
\begin{eqnarray}
p_{j} = \Phi(w_{1} x_{j} - p_{j-1}) + p_{j-1}
\end{eqnarray}

and

\begin{eqnarray}
\Phi(x) =
        \begin{cases}
        x, x > 0 \\
        0, -1 < x < 0 \\
        x-1, x < -1 \\
        \end{cases}

\end{eqnarray}

Using Chain Rule, we obtain
\begin{eqnarray}
\frac{\partial y_{j}}{\partial x_{j}} &=& \frac{\partial y_{j}}{\partial p_{j}} \frac{\partial p_{j}}{\partial x_{j}} \\
                                      &=& \sum_{i=1}^{S} \tilde{\theta_{i}} \frac{\partial \tanh(\theta_{i} p_{j} + \theta_{i0})}{\partial p_{j}} \frac{\partial{\Phi(w^{1} x_{j} - p_{j-1})}}{\partial{x_{j}}}
\end{eqnarray}

                                      # &=& \begin{cases}
                                      # 0, -1 < w_{1} x_{j} - p_{j-1} < 0 \\
                                      # \sum_{i=1}^{S} \tilde{\theta_{i}} \theta_{i} (1 - \tanh^{2}(\theta_{i} p_{j} + \theta_{i0})) w^{1}, \text{otherwise}
                                      # \end{cases}


To consider *multiple plays* case, we reformulate the derivation as following:

\begin{eqnarray}
\frac{\partial {y_{j}^{1}}}{\partial x_{j}} &=& \frac{\partial{y_{j}^{1}}}{\partial{p_{j}^{1}}} \frac{\partial{ p_{j}}^{1}}{\partial x_{j}} \\
                                      &=& \sum_{i=1}^{S} \tilde{\theta_{i}^{1}} \frac{\partial \tanh(\theta_{i}^{1} p_{j}^{1} + \theta_{i0})}{\partial p_{j}^{1}} \frac{\partial{\Phi(w^{1} x_{j} - p_{j-1}^{1})}}{\partial{x_{j}}} \\
\end{eqnarray}
#                                       &=& \begin{cases}
#                                       0, -1 < w_{1} x_{j} - p_{j-1} < 0 \\
#                                       \sum_{i=1}^{S} \tilde{\theta_{i}^{1}} \theta_{i}^{1} (1 - \tanh^{2}(\theta_{i}^{1} p_{j}^{1} + \theta_{i0}^{1})) w^{1}, \text{otherwise}
#                                       \end{cases}


Now from the architecture, we know that if we have \(P\) plays,
\begin{eqnarray}
F = \frac{1}{P} \sum_{i=1}^{P} G^{i}
\end{eqnarray}
Where \(F=[f_1, f_2, ..., f_n]\),
and
\begin{eqnarray}
f_{j} = \frac{1}{P} \sum_{i=1}^{P} y_{j}^{i}
\end{eqnarray}

our derivation is:

\begin{eqnarray}
\frac{\partial f_{j}}{\partial x_{j}} &=& \frac{1}{P} \sum_{k=1}^{P} \frac{\partial {{y_{j}^{k}}}}{\partial {{x_{j}}}} \\
               &=& \frac{1}{P} \sum_{k=1}^{P} \frac{\partial {y_{j}^{k}}}{\partial {p_{j}^{k}}} \frac{\partial {p_{j}^{k}}}{\partial {x_{j}}} \\
               &=& \frac{1}{P} \sum_{k=1}^{P}  \sum_{i=1}^{S} \tilde{\theta_{i}^{k}} \frac{\partial \tanh(\theta_{i}^{k} p_{j}^{k} + \theta_{i0})}{\partial p_{j}^{k}} \frac{\partial{\Phi(w^{k} x_{j} - p_{j-1}^{k})}}{\partial{x_{j}}} \\
\end{eqnarray}
               # &=&                        \frac{1}{P} \sum_{k=1}^{P}  \sum_{i=1}^{S} \tilde{\theta_{i}^{k}} \theta_{i}^{k} (1 - \tanh^{2}(\theta_{i}^{k} p_{j}^{k} + \theta_{i0}^{k})) w^{k}
